ExistentialRules/ChaseSequence/CoreChase/AuxiliarySeq.lean
@@ -1,98 +1,102 @@
-import ExistentialRules.ChaseSequence.ChaseBranch
-import ExistentialRules.Models.Basic
-import ExistentialRules.Models.Cores
-import PossiblyInfiniteTrees.PossiblyInfiniteTree.FiniteDegreeTree.Basic
-import ExistentialRules.Models.Basic
-import ExistentialRules.Triggers.Basic
-import ExistentialRules.AtomsAndFacts.Basic
-import ExistentialRules.AtomsAndFacts.SubstitutionsAndHomomorphisms
-import ExistentialRules.ChaseSequence.Termination.Basic
-import ExistentialRules.ChaseSequence.Universality
+/-
+Copyright 2026 Henrik Tscherny, Lukas Gerlach
+Released under Apache 2.0 license as described in the file LICENSE.
+-/
 
+module
+
+public import ExistentialRules.ChaseSequence.ChaseBranch
 import ExistentialRules.ChaseSequence.Deterministic
 
-import ExistentialRules.ChaseSequence.CoreChase.Homomorphisms
-import ExistentialRules.ChaseSequence.CoreChase.Triggers
-import ExistentialRules.ChaseSequence.CoreChase.Termination
+import ExistentialRules.ChaseSequence.CoreChase.Basic
+public import ExistentialRules.ChaseSequence.CoreChase.CoreChaseBranch
 
+/-!
+# The Core Chase terminates if a finite universal model exists
+
+In this file, we aim to show the result from the title.
+THIS IS EXTREMELY PRELIMINARY. A lot of things are still open here.
+-/
 
 variable {sig : Signature} [DecidableEq sig.P] [DecidableEq sig.C] [DecidableEq sig.V]
-variable {kb : KnowledgeBase sig}
-
 
 namespace CoreChaseBranch
 
-  theorem exTerminatingCoreChaseBranchIfExTerminatingChaseBranch (scb : RegularChaseBranch obs kb) (scb_term : scb.terminates) :
-      ∃ (ccb : CoreChaseBranch kb), ccb.terminates := by
-    -- the idea would be to build the core chase branch directly from the restricted chase branch by dropping the nodes whose triggers are no longer active after core computation; the construction is not trivial though
-    sorry
+variable {kb : KnowledgeBase sig}
 
-  theorem existsNonTerminatingChaseBranchIfExistsNonTerminatingCoreChaseBranch (ccb : CoreChaseBranch kb) (ccb_term : ¬ ccb.terminates) : ∃ (scb : RegularChaseBranch obs kb), ¬ scb.terminates := by
-    sorry
+theorem exTerminatingCoreChaseBranchIfExTerminatingChaseBranch (scb : RegularChaseBranch obs kb) (scb_term : scb.terminates) :
+    ∃ (ccb : CoreChaseBranch kb), ccb.terminates := by
+  -- the idea would be to build the core chase branch directly from the restricted chase branch by dropping the nodes whose triggers are no longer active after core computation; the construction is not trivial though
+  sorry
 
-  theorem exTerminatingCoreChaseBranchIfExFiniteUniversalModel (ccb : CoreChaseBranch kb) (kb_det : kb.isDeterministic) : (∃ (fs : FactSet sig), fs.finite ∧ fs.universallyModelsKb kb) → ccb.terminates := by
+theorem existsNonTerminatingChaseBranchIfExistsNonTerminatingCoreChaseBranch (ccb : CoreChaseBranch kb) (ccb_term : ¬ ccb.terminates) :
+    ∃ (scb : RegularChaseBranch (RestrictedObsolescence sig) kb), ¬ scb.terminates := by
+  sorry
 
-    /-
-    ccb : A_0 → A_1 → A_2 .....
-    scb : B_1 → B_2 → B_3 .....
-                B_n
-    -/
+public theorem exTerminatingCoreChaseBranchIfExFiniteUniversalModel (ccb : CoreChaseBranch kb) (kb_det : kb.isDeterministic) :
+    (∃ (fs : FactSet sig), fs.finite ∧ fs.universallyModelsKb kb) → ccb.terminates := by
 
-    intro ⟨M, ⟨M_list, _, M_eq⟩, M_umod⟩
+  /-
+  ccb : A_0 → A_1 → A_2 .....
+  scb : B_1 → B_2 → B_3 .....
+              B_n
+  -/
 
-    apply Classical.byContradiction
-    intro contra
+  intro ⟨M, ⟨M_list, _, M_eq⟩, M_umod⟩
 
-    have ex_inf_scb := existsNonTerminatingChaseBranchIfExistsNonTerminatingCoreChaseBranch ccb contra
-    rcases ex_inf_scb with ⟨scb, scb_non_term⟩
+  apply Classical.byContradiction
+  intro contra
 
-    -- R = B^{res}_ω
-    let R := scb.result
+  have ex_inf_scb := existsNonTerminatingChaseBranchIfExistsNonTerminatingCoreChaseBranch ccb contra
+  rcases ex_inf_scb with ⟨scb, scb_non_term⟩
 
-    have R_umod : R.universallyModelsKb kb := scb.deterministicChaseBranchResultUniversallyModelsKb kb_det
+  -- R = B^{res}_ω
+  let R := scb.result
 
-    have hom_M_R : ∃ (h : GroundTermMapping sig), h.isHomomorphism M R := by
-      rcases M_umod with ⟨M_umod_l, M_umod_r⟩
-      specialize M_umod_r R RegularChaseBranch.result_models_kb
-      exact M_umod_r
+  have R_umod : R.universallyModelsKb kb := scb.deterministicChaseBranchResultUniversallyModelsKb kb_det
 
-    have hom_R_M : ∃ (h : GroundTermMapping sig), h.isHomomorphism R M := by
-      rcases R_umod with ⟨R_umod_l, R_umod_r⟩
-      specialize R_umod_r M M_umod.left
-      exact R_umod_r
+  have hom_M_R : ∃ (h : GroundTermMapping sig), h.isHomomorphism M R := by
+    rcases M_umod with ⟨M_umod_l, M_umod_r⟩
+    specialize M_umod_r R RegularChaseBranch.result_models_kb
+    exact M_umod_r
 
-    rcases hom_M_R with ⟨h_M_R, hom_M_R⟩
-    rcases hom_R_M with ⟨h_R_M, hom_R_M⟩
+  have hom_R_M : ∃ (h : GroundTermMapping sig), h.isHomomorphism R M := by
+    rcases R_umod with ⟨R_umod_l, R_umod_r⟩
+    specialize R_umod_r M M_umod.left
+    exact R_umod_r
 
-    rcases RegularChaseDerivationSkeleton.facts_mem_some_node_of_mem_result (M_list.map h_M_R.applyFact) (by
-      intro f f_mem; apply hom_M_R.right; rw [GroundTermMapping.mem_applyFactSet]
-      rw [List.mem_toSet, List.mem_map] at f_mem; rcases f_mem with ⟨e, e_mem, f_eq⟩
-      exists e; rw [← M_eq, f_eq]; exact ⟨e_mem, rfl⟩)
-    with ⟨node, node_mem, M_sub_node⟩
+  rcases hom_M_R with ⟨h_M_R, hom_M_R⟩
+  rcases hom_R_M with ⟨h_R_M, hom_R_M⟩
 
-    have hom_M_node : h_M_R.isHomomorphism M node.facts := by
-      constructor; exact hom_M_R.left
-      intro f f_mem
-      apply M_sub_node
-      rw [List.mem_toSet, List.mem_map]
-      rw [GroundTermMapping.mem_applyFactSet] at f_mem; rcases f_mem with ⟨e, e_mem, f_eq⟩
-      exists e; rw [M_eq, f_eq]; exact ⟨e_mem, rfl⟩
+  rcases RegularChaseDerivationSkeleton.facts_mem_some_node_of_mem_result (M_list.map h_M_R.applyFact) (by
+    intro f f_mem; apply hom_M_R.right; rw [GroundTermMapping.mem_applyFactSet]
+    rw [List.mem_toSet, List.mem_map] at f_mem; rcases f_mem with ⟨e, e_mem, f_eq⟩
+    exists e; rw [← M_eq, f_eq]; exact ⟨e_mem, rfl⟩)
+  with ⟨node, node_mem, M_sub_node⟩
 
-    have hom_node_M : h_R_M.isHomomorphism node.facts M := by
-      constructor; exact hom_R_M.left
-      intro f f_mem
-      apply hom_R_M.right
-      apply h_R_M.apply_generalized_atom_set_subset_of_subset _ _ (RegularChaseDerivationSkeleton.facts_node_subset_result node node_mem)
-      exact f_mem
+  have hom_M_node : h_M_R.isHomomorphism M node.facts := by
+    constructor; exact hom_M_R.left
+    intro f f_mem
+    apply M_sub_node
+    rw [List.mem_toSet, List.mem_map]
+    rw [GroundTermMapping.mem_applyFactSet] at f_mem; rcases f_mem with ⟨e, e_mem, f_eq⟩
+    exists e; rw [M_eq, f_eq]; exact ⟨e_mem, rfl⟩
 
-    have node_finite := scb.facts_finite_of_mem ⟨node, node_mem⟩
+  have hom_node_M : h_R_M.isHomomorphism node.facts M := by
+    constructor; exact hom_R_M.left
+    intro f f_mem
+    apply hom_R_M.right
+    apply h_R_M.apply_generalized_atom_set_subset_of_subset _ _ (RegularChaseDerivationSkeleton.facts_node_subset_result node node_mem)
+    exact f_mem
 
-    rcases node.facts.exists_weak_core_for_set_of_finite node_finite with ⟨node_core, node_core_isCore⟩
+  have node_finite := scb.facts_finite_of_mem ⟨node, node_mem⟩
 
-    -- the rest of the prove shall take scb up until node and then compute the core once
-    -- we need to prove that a regular core chase branch with the same result exists (this could be a general theorem, i.e. computing the core after any finite number of steps does not make a difference for the result)
-    -- then we need to argue that the result of this core chase branch is isomorphic to M (basically since node_core is isomorphic to M) and then we need to argue that the isomorphism preserves modelhood, i.e. that the result of the core chase branch is a model, which justifies that the core chase branch ends at this point. This also yields the desired contradiction.
+  rcases node.facts.exists_weak_core_for_set_of_finite node_finite with ⟨node_core, node_core_isCore⟩
 
-    sorry
+  -- the rest of the prove shall take scb up until node and then compute the core once
+  -- we need to prove that a regular core chase branch with the same result exists (this could be a general theorem, i.e. computing the core after any finite number of steps does not make a difference for the result)
+  -- then we need to argue that the result of this core chase branch is isomorphic to M (basically since node_core is isomorphic to M) and then we need to argue that the isomorphism preserves modelhood, i.e. that the result of the core chase branch is a model, which justifies that the core chase branch ends at this point. This also yields the desired contradiction.
+
+  sorry
 
 end CoreChaseBranch
