ExistentialRules/ChaseSequence/CoreChase/CoreChaseNode.lean
@@ -46,5 +46,72 @@ theorem outgoingFacts_eq {node : CoreChaseNode rules} : coreChaseNodeInstance.ou
 theorem out_sub_in : coreChaseNodeInstance.out_sub_in (N := CoreChaseNode rules) := by
   intro node f; rw [ingoingFacts_eq, outgoingFacts_eq]; exact node.homSubset.left f
 
+/-- The origin trigger of a `CoreChaseNode` is inactive for each homSubset of the node's facts, given that this subset is finite. -/
+theorem origin_trg_inactive_of_isWeakCore_of_homSubset_of_finite
+    {node : CoreChaseNode rules} {fs : FactSet sig} (wc : fs.isWeakCore) (homSub : fs.homSubset node.facts) (fin : fs.finite) :
+    ∀ orig ∈ node.origin, ¬ orig.fst.val.active fs := by
+  intro orig orig_mem ⟨loaded, contra⟩
+  apply contra
+
+  let idx : Fin orig.fst.val.rule.head.length := ⟨orig.snd.val, by rw [← PreTrigger.length_mapped_head]; exact orig.snd.isLt⟩
+  exists idx
+
+  -- the origin trigger of our node is satisfied on on the node's facts
+  have orig_trg_satisfied_on_facts : orig.fst.val.satisfied_for_disj node.facts idx := by
+    apply PreTrigger.satisfied_for_disj_of_mapped_head_contained
+    apply node.facts_contain_origin_result
+    exact orig_mem
+  rcases orig_trg_satisfied_on_facts with ⟨subs, satisfied⟩
+
+  -- we have a homomorphism from node.facts to fs; because of fs is a homSubset of node.facts, it is even an endomorphism on fs
+  rcases homSub.right with ⟨h, hom⟩
+  have h_endo : h.isHomomorphism fs fs := by
+    constructor; exact hom.left
+    apply Set.subset_trans _ hom.right
+    apply TermMapping.apply_generalized_atom_set_subset_of_subset
+    exact homSub.left
+
+  -- we can repeat the homomorphism often enough such that it is the id on all terms in cd.head.core; this works since fs is finite and a core
+  have node_strong_core : fs.isStrongCore := fs.isStrongCore_of_isWeakCore_of_finite wc fin
+  have endo_surj : h.surjectiveSet fs.terms fs.terms := (node_strong_core h h_endo).right.right
+  rcases fs.terms_finite_of_finite fin with ⟨terms, _, terms_eq⟩
+  have terms_eq : ∀ t, t ∈ fs.terms ↔ t ∈ terms := by intro _; rw [terms_eq]
+  rw [Function.surjective_set_list_equiv terms_eq terms_eq] at endo_surj
+  rcases h.exists_repetition_that_is_inverse_of_surj terms endo_surj with ⟨k, inv⟩
+
+  let target_h : GroundTermMapping sig := (h.repeat_fun k) ∘ h
+  have target_h_hom : target_h.isHomomorphism node.facts fs := by
+    apply GroundTermMapping.isHomomorphism_compose; exact hom; exact GroundTermMapping.repeat_isHomomorphism h_endo k
+  have target_h_id_terms : ∀ t ∈ terms, target_h t = t := inv
+
+  -- we can use the repeated homomorphism together with the substitution that witnesses satisfaction to see that the trigger is also satisfied in fs but this yields exactly the contridiction that we were looking for
+  exists target_h ∘ subs; constructor
+  . intro v v_mem; rw [Function.comp_apply, satisfied.left v v_mem, target_h_id_terms]
+    rw [← terms_eq]
+    apply FactSet.terms_subset_of_subset loaded
+    rw [FactSet.mem_terms_toSet]
+    rw [PreTrigger.mem_terms_mapped_body_iff]; apply Or.inr
+    exists v; constructor
+    . apply Rule.frontier_subset_vars_body; exact v_mem
+    . rfl
+  . rw [GroundSubstitution.apply_function_free_conj_compose_of_isIdOnConstants _ _ target_h_hom.left]
+    intro f f_mem
+    rw [List.mem_toSet, Function.comp_apply, TermMapping.mem_apply_generalized_atom_list] at f_mem
+    rcases f_mem with ⟨intermediate, intermediate_mem, f_eq⟩
+    apply target_h_hom.right
+    rw [f_eq]
+    apply TermMapping.apply_generalized_atom_mem_apply_generalized_atom_set
+    apply satisfied.right
+    rw [List.mem_toSet]
+    exact intermediate_mem
+
+/-- The origin trigger of a `CoreChaseNode` is inactive on the node's core. -/
+theorem origin_trg_inactive_for_own_core_of_finite {node : CoreChaseNode rules} (fin : node.core.finite) :
+    ∀ orig ∈ node.origin, ¬ orig.fst.val.active node.core := by
+  apply origin_trg_inactive_of_isWeakCore_of_homSubset_of_finite
+  . exact node.isWeakCore
+  . exact node.homSubset
+  . exact fin
+
 end CoreChaseNode
 
